declared some arguments maximally implicit, and started to replace Add [Parametric] Morphism and Add Relation by Instance, and Implicit Arguments by Arguments

trunk/color/SemLab/ASemLab.v
@@ -16,420 +16,427 @@ Require Import ATrs AInterpretation BoolUtil LogicUtil EqUtil VecUtil SN
 
 Section S.
 
-Variable Sig : Signature.
+  Variable Sig : Signature.
 
-Notation term := (term Sig). Notation terms := (vector term).
-Notation rule := (rule Sig). Notation rules := (rules Sig).
+  Notation term := (term Sig). Notation terms := (vector term).
+  Notation rule := (rule Sig). Notation rules := (rules Sig).
 
 (***********************************************************************)
 (** labels *)
 
-Variable L : Sig -> Type.
-Variable beq : forall f g, L f -> L g -> bool.
-Variable beq_ok : forall f (l m : L f), beq l m = true <-> l = m.
+  Variable L : Sig -> Type.
+  Variable beq : forall f g, L f -> L g -> bool.
+  Variable beq_ok : forall f (l m : L f), beq l m = true <-> l = m.
 
 (***********************************************************************)
 (** labelled signature *)
 
-Variable I : interpretation Sig.
+  Variable I : interpretation Sig.
 
-Notation int := (@term_int _ I).
+  Notation int := (@term_int _ I).
 
-Record lab_symb : Type := mk {
-  l_symb : Sig;
-  l_lab : L l_symb }.
+  Record lab_symb : Type := mk {
+    l_symb : Sig;
+    l_lab : L l_symb }.
 
-Notation eq_symb_dec := (@eq_symb_dec Sig).
+  Notation eq_symb_dec := (@eq_symb_dec Sig).
 
-Ltac Leqtac := repeat
-  match goal with
-    | H : @mk ?x _ = @mk ?x _ |- _ =>
-      let h1 := fresh in
-        (injection H; intro h1; ded (inj_pairT2 eq_symb_dec h1);
-          clear h1; clear H)
-    | H : @mk _ _ = @mk _ _ |- _ =>
-      let h1 := fresh in let h2 := fresh in
-        (injection H; clear H; intros h1 h2; subst;
-          ded (inj_pairT2 eq_symb_dec h1); clear h1; subst)
-  end.
+  Ltac Leqtac := repeat
+    match goal with
+      | H : @mk ?x _ = @mk ?x _ |- _ =>
+        let h1 := fresh in
+          (injection H; intro h1; ded (inj_pairT2 eq_symb_dec h1);
+            clear h1; clear H)
+      | H : @mk _ _ = @mk _ _ |- _ =>
+        let h1 := fresh in let h2 := fresh in
+          (injection H; clear H; intros h1 h2; subst;
+            ded (inj_pairT2 eq_symb_dec h1); clear h1; subst)
+    end.
 
-Definition beq_lab_symb (fl1 fl2 : lab_symb) :=
-  let (f1,l1) := fl1 in let (f2,l2) := fl2 in beq_symb f1 f2 && beq l1 l2.
+  Definition beq_lab_symb (fl1 fl2 : lab_symb) :=
+    let (f1,l1) := fl1 in let (f2,l2) := fl2 in beq_symb f1 f2 && beq l1 l2.
 
-Lemma beq_lab_symb_ok : forall fl1 fl2,
-  beq_lab_symb fl1 fl2 = true <-> fl1 = fl2.
+  Lemma beq_lab_symb_ok : forall fl1 fl2,
+    beq_lab_symb fl1 fl2 = true <-> fl1 = fl2.
 
-Proof.
-intros [f1 l1] [f2 l2]. simpl. split; intro. rewrite andb_eq in H. destruct H.
-rewrite beq_symb_ok in H. subst. rewrite beq_ok in H0. subst. refl.
-Leqtac. rewrite andb_eq. rewrite (beq_refl (@beq_symb_ok Sig)).
-rewrite beq_ok. auto.
-Qed.
+  Proof.
+    intros [f1 l1] [f2 l2]. simpl. split; intro. rewrite andb_eq in H.
+    destruct H.
+    rewrite beq_symb_ok in H. subst. rewrite beq_ok in H0. subst. refl.
+    Leqtac. rewrite andb_eq. rewrite (beq_refl (@beq_symb_ok Sig)).
+    rewrite beq_ok. auto.
+  Qed.
 
-Definition lab_arity (fl : lab_symb) := let (f,_) := fl in arity f.
+  Definition lab_arity (fl : lab_symb) := let (f,_) := fl in arity f.
 
-Definition lab_sig := mkSignature lab_arity beq_lab_symb_ok.
+  Definition lab_sig := mkSignature lab_arity beq_lab_symb_ok.
 
-Notation Sig' := lab_sig. Notation Fun' := (@Fun Sig').
-Notation term' := (ATerm.term Sig'). Notation terms' := (vector term').
-Notation rule' := (ATrs.rule Sig'). Notation rules' := (rules Sig').
+  Notation Sig' := lab_sig. Notation Fun' := (@Fun Sig').
+  Notation term' := (ATerm.term Sig'). Notation terms' := (vector term').
+  Notation rule' := (ATrs.rule Sig'). Notation rules' := (rules Sig').
 
 (***********************************************************************)
 (** labelling *)
 
-Variable pi : forall f : Sig, vector I (arity f) -> L f.
+  Variable pi : forall f : Sig, vector I (arity f) -> L f.
 
-Fixpoint lab v t :=
-  match t with
-    | Var x => Var x
-    | Fun f ts => Fun' (mk (pi f (Vmap (int v) ts))) (Vmap (lab v) ts)
-  end.
+  Fixpoint lab v t :=
+    match t with
+      | Var x => Var x
+      | Fun f ts => Fun' (mk (pi f (Vmap (int v) ts))) (Vmap (lab v) ts)
+    end.
 
-Definition lab_rule v (a : rule) :=
-  let (l,r) := a in mkRule (lab v l) (lab v r).
+  Definition lab_rule v (a : rule) :=
+    let (l,r) := a in mkRule (lab v l) (lab v r).
 
-Definition lab_rules R a := exists b, exists v, R b /\ a = lab_rule v b.
+  Definition lab_rules R a := exists b, exists v, R b /\ a = lab_rule v b.
 
-Definition lab_sub v s (x : variable) := lab v (s x).
+  Definition lab_sub v s (x : variable) := lab v (s x).
 
-Notation "f 'o' g" := (fun x => f (g x)) (at level 70).
+  Notation "f 'o' g" := (fun x => f (g x)) (at level 70).
 
-Lemma lab_sub_eq : forall v s t,
-  lab v (sub s t) = sub (lab_sub v s) (lab (beta v s) t).
+  Lemma lab_sub_eq : forall v s t,
+    lab v (sub s t) = sub (lab_sub v s) (lab (beta v s) t).
 
-Proof.
-intros v s t. pattern t; apply term_ind with (Q := fun n (ts : terms n) =>
-  Vmap (lab v o sub s) ts = Vmap (sub (lab_sub v s) o lab (beta v s)) ts);
-  clear t; intros; simpl.
-(* Var *)
-unfold lab_sub. refl.
-(* Fun *)
-repeat rewrite Vmap_map. rewrite Vmap_eq_ext with (g := int (beta v s)).
-2: apply substitution_lemma. apply args_eq. hyp.
-(* Vnil *)
-refl.
-(* Vcons *)
-apply Vcons_eq_intro; hyp.
-Qed.
+  Proof.
+    intros v s t. pattern t; apply term_ind with (Q := fun n (ts : terms n) =>
+    Vmap (lab v o sub s) ts = Vmap (sub (lab_sub v s) o lab (beta v s)) ts);
+    clear t; intros; simpl.
+    (* Var *)
+    unfold lab_sub. refl.
+    (* Fun *)
+    repeat rewrite Vmap_map. rewrite Vmap_eq_ext with (g := int (beta v s)).
+    2: apply substitution_lemma. apply args_eq. hyp.
+    (* Vnil *)
+    refl.
+    (* Vcons *)
+    apply Vcons_eq_intro; hyp.
+  Qed.
 
-Require Import VecMax.
+  Require Import VecMax.
 
-Lemma lab_fval : forall v t n, n > maxvar t -> lab (fval v n) t = lab v t.
+  Lemma lab_fval : forall v t n, n > maxvar t -> lab (fval v n) t = lab v t.
 
-Proof.
-intros v t. pattern t; apply term_ind with (Q := fun n (ts : terms n) =>
-  forall n, n > maxvars ts -> Vmap (lab v) ts = Vmap (lab (fval v n)) ts);
-  clear t; simpl; intros.
-(* Var *)
-refl.
-(* Fun *)
-rewrite (H n). assert (Vmap (int v) v0 = Vmap (int (fval v n)) v0).
-apply Vmap_eq. apply Vforall_intro. intros. apply term_int_eq_fval_lt.
-apply le_lt_trans with (Vmax (Vmap (@maxvar Sig) v0)). apply Vmax_in.
-apply Vin_map_intro. hyp. hyp. rewrite H1. refl. unfold maxvars. omega.
-(* Vnil *)
-refl.
-(* Vcons *)
-rewrite maxvars_cons in H1. rewrite gt_max in H1. destruct H1.
-rewrite (H0 n0). 2: hyp. rewrite (H n0). 2: hyp. refl.
-Qed.
+  Proof.
+    intros v t. pattern t; apply term_ind with (Q := fun n (ts : terms n) =>
+    forall n, n > maxvars ts -> Vmap (lab v) ts = Vmap (lab (fval v n)) ts);
+    clear t; simpl; intros.
+    (* Var *)
+    refl.
+    (* Fun *)
+    rewrite (H n). assert (Vmap (int v) v0 = Vmap (int (fval v n)) v0).
+    apply Vmap_eq. apply Vforall_intro. intros. apply term_int_eq_fval_lt.
+    apply le_lt_trans with (Vmax (Vmap (@maxvar Sig) v0)). apply Vmax_in.
+    apply Vin_map_intro. hyp. hyp. rewrite H1. refl. unfold maxvars. omega.
+    (* Vnil *)
+    refl.
+    (* Vcons *)
+    rewrite maxvars_cons in H1. rewrite gt_max in H1. destruct H1.
+    rewrite (H0 n0). 2: hyp. rewrite (H n0). 2: hyp. refl.
+  Qed.
 
-Lemma lab_rule_fval : forall v a n,
-  n > maxvar_rule a -> lab_rule (fval v n) a = lab_rule v a.
+  Lemma lab_rule_fval : forall v a n,
+    n > maxvar_rule a -> lab_rule (fval v n) a = lab_rule v a.
 
-Proof.
-intros v [l r] n. simpl. rewrite gt_max. intuition.
-rewrite lab_fval. 2: hyp. rewrite lab_fval. 2: hyp. refl.
-Qed.
+  Proof.
+    intros v [l r] n. simpl. rewrite gt_max. intuition.
+    rewrite lab_fval. 2: hyp. rewrite lab_fval. 2: hyp. refl.
+  Qed.
 
-Notation fold_max := (@fold_max Sig).
+  Notation fold_max := (@fold_max Sig).
 
-Require Import Max.
+  Require Import Max.
 
-Lemma map_lab_rule_fval : forall v R n, n > maxvar_rules R ->
-  map (lab_rule (fval v n)) R = map (lab_rule v) R.
+  Lemma map_lab_rule_fval : forall v R n, n > maxvar_rules R ->
+    map (lab_rule (fval v n)) R = map (lab_rule v) R.
 
-Proof.
-induction R; simpl; intros. refl. unfold maxvar_rules in H. simpl in H.
-rewrite lab_rule_fval. rewrite IHR. refl.
-apply le_lt_trans with (fold_left fold_max R (fold_max 0 a)).
-apply maxvar_rules_init_mon. apply le_max_l. hyp.
-apply le_lt_trans with (fold_left fold_max R (fold_max 0 a)).
-apply maxvar_rules_init. hyp.
-Qed.
+  Proof.
+    induction R; simpl; intros. refl. unfold maxvar_rules in H. simpl in H.
+    rewrite lab_rule_fval. rewrite IHR. refl.
+    apply le_lt_trans with (fold_left fold_max R (fold_max 0 a)).
+    apply maxvar_rules_init_mon. apply le_max_l. hyp.
+    apply le_lt_trans with (fold_left fold_max R (fold_max 0 a)).
+    apply maxvar_rules_init. hyp.
+  Qed.
 
 (***********************************************************************)
 (** ordering of labels *)
 
-Variable Lgt : forall f, relation (L f). Infix ">L" := Lgt (at level 50).
+  Variable Lgt : forall f, relation (L f). Infix ">L" := Lgt (at level 50).
 
-Let Lge f := @Lgt f %. Infix ">=L" := Lge (at level 50).
+  Let Lge f := @Lgt f %. Infix ">=L" := Lge (at level 50).
 
-Definition Fun'_vars f (a : L f) := Fun' (mk a) (fresh_vars (arity f)).
+  Definition Fun'_vars f (a : L f) := Fun' (mk a) (fresh_vars (arity f)).
 
-Definition decr f (a b : L f) := mkRule (Fun'_vars a) (Fun'_vars b).
+  Definition decr f (a b : L f) := mkRule (Fun'_vars a) (Fun'_vars b).
 
-Definition Decr (rho : rule') :=
-  exists f, exists a : L f, exists b, a >L b /\ rho = decr a b.
+  Definition Decr (rho : rule') :=
+    exists f, exists a : L f, exists b, a >L b /\ rho = decr a b.
 
-Lemma Lge_Decr : forall f (ts : terms' (arity f)) (a b : L f),
-  a >=L b -> red Decr # (Fun' (mk a) ts) (Fun' (mk b) ts).
+  Lemma Lge_Decr : forall f (ts : terms' (arity f)) (a b : L f),
+    a >=L b -> red Decr # (Fun' (mk a) ts) (Fun' (mk b) ts).
 
-Proof.
-intros. destruct H. subst. apply rt_refl. apply rt_step.
-exists (Fun'_vars a). exists (Fun'_vars b). exists Hole.
-exists (sub_vars ts). simpl. intuition.
-exists f. exists a. exists b. intuition.
-apply args_eq. apply sub_fresh_vars.
-apply args_eq. apply sub_fresh_vars.
-Qed.
+  Proof.
+    intros. destruct H. subst. apply rt_refl. apply rt_step.
+    exists (Fun'_vars a). exists (Fun'_vars b). exists Hole.
+    exists (sub_vars ts). simpl. intuition.
+    exists f. exists a. exists b. intuition.
+    apply args_eq. apply sub_fresh_vars.
+    apply args_eq. apply sub_fresh_vars.
+  Qed.
 
 (***********************************************************************)
 (** unlabelling *)
 
-Require Import AMorphism.
+  Require Import AMorphism.
 
-Definition F (f' : Sig') := let (f,_) := f' in f.
+  Definition F (f' : Sig') := let (f,_) := f' in f.
 
-Lemma HF : forall f', arity f' = arity (F f').
+  Lemma HF : forall f', arity f' = arity (F f').
 
-Proof.
-intros (f,l). refl.
-Qed.
+  Proof. intros (f,l). refl. Qed.
 
-Definition unlab := Ft HF.
-Definition unlab_rules := Frs HF.
-Definition unlab_rules_fin := Fl HF.
+  Definition unlab := Ft HF.
+  Definition unlab_rules := Frs HF.
+  Definition unlab_rules_fin := Fl HF.
 
-Lemma Ft_epi : forall v t, unlab (lab v t) = t.
+  Lemma Ft_epi : forall v t, unlab (lab v t) = t.
 
-Proof.
-intros v t. pattern t. apply term_ind with (Q := fun n (ts : terms n) =>
-  Vmap (unlab o lab v) ts = ts); clear t; intros; simpl.
-refl. apply args_eq. rewrite Vmap_map. rewrite H. apply Vcast_refl.
-refl. rewrite H. rewrite H0. refl.
-Qed.
+  Proof.
+    intros v t. pattern t. apply term_ind with (Q := fun n (ts : terms n) =>
+    Vmap (unlab o lab v) ts = ts); clear t; intros; simpl.
+    refl. apply args_eq. rewrite Vmap_map. rewrite H. apply Vcast_refl.
+    refl. rewrite H. rewrite H0. refl.
+  Qed.
 
-Lemma Frs_iso : forall R, unlab_rules (lab_rules R) [=] R.
+  Lemma Frs_iso : forall R, unlab_rules (lab_rules R) [=] R.
 
-Proof.
-intros R [l r]. split.
-(* [= *)
-intros [[l' r'] [h1 h2]]. destruct h1 as [[x y] [v [h h']]]. inversion h'.
-inversion h2. subst. repeat rewrite Ft_epi. hyp.
-(* =] *)
-unfold Frs. intro. set (v := fun x : variable => some_elt I).
-exists (mkRule (lab v l) (lab v r)). split.
-unfold lab_rules. exists (mkRule l r). exists v. intuition.
-simpl. repeat rewrite Ft_epi. refl.
-Qed.
+  Proof.
+    intros R [l r]. split.
+    (* [= *)
+    intros [[l' r'] [h1 h2]]. destruct h1 as [[x y] [v [h h']]]. inversion h'.
+    inversion h2. subst. repeat rewrite Ft_epi. hyp.
+    (* =] *)
+    unfold Frs. intro. set (v := fun x : variable => some_elt I).
+    exists (mkRule (lab v l) (lab v r)). split.
+    unfold lab_rules. exists (mkRule l r). exists v. intuition.
+    simpl. repeat rewrite Ft_epi. refl.
+  Qed.
 
-Lemma red_Frs_Decr : red (unlab_rules Decr) << @eq term.
+  Lemma red_Frs_Decr : red (unlab_rules Decr) << @eq term.
 
-Proof.
-intros t u h. redtac. subst. destruct lr as [[l' r'] [h1 h2]].
-destruct h1 as [f [a [b [ab h]]]]. inversion h. subst. inversion h2.
-assert (HF (mk a) = HF (mk b)). apply UIP. apply eq_nat_dec. rewrite H. refl.
-Qed.
+  Proof.
+    intros t u h. redtac. subst. destruct lr as [[l' r'] [h1 h2]].
+    destruct h1 as [f [a [b [ab h]]]]. inversion h. subst. inversion h2.
+    assert (HF (mk a) = HF (mk b)). apply UIP. apply eq_nat_dec. rewrite H.
+    refl.
+  Qed.
 
-Lemma rt_red_Frs_Decr : red (unlab_rules Decr) # << @eq term.
+  Lemma rt_red_Frs_Decr : red (unlab_rules Decr) # << @eq term.
 
-Proof.
-intros t u. induction 1. apply red_Frs_Decr. hyp. refl. trans y; hyp.
-Qed.
+  Proof.
+    intros t u. induction 1. apply red_Frs_Decr. hyp. refl. trans y; hyp.
+  Qed.
 
-Lemma red_mod_Frs_Decr : forall E,
-  red (unlab_rules (Decr ++ lab_rules E)) << red E %.
+  Lemma red_mod_Frs_Decr : forall E,
+    red (unlab_rules (Decr ++ lab_rules E)) << red E %.
 
-Proof.
-intros E t u h. redtac. subst. apply Frs_app in lr. destruct lr.
-left. eapply rt_red_Frs_Decr. apply rt_step. apply red_rule. hyp.
-right. apply red_rule. do 2 destruct H. rewrite H0. clear H0. do 3 destruct H.
-subst. destruct x0. simpl. repeat rewrite Ft_epi. hyp.
-Qed.
+  Proof.
+    intros E t u h. redtac. subst. apply Frs_app in lr. destruct lr.
+    left. eapply rt_red_Frs_Decr. apply rt_step. apply red_rule. hyp.
+    right. apply red_rule. do 2 destruct H. rewrite H0. clear H0.
+    do 3 destruct H.
+    subst. destruct x0. simpl. repeat rewrite Ft_epi. hyp.
+  Qed.
 
-Lemma rt_red_mod_Frs_Decr : forall E,
-  red (unlab_rules (Decr ++ lab_rules E)) # << red E #.
+  Lemma rt_red_mod_Frs_Decr : forall E,
+    red (unlab_rules (Decr ++ lab_rules E)) # << red E #.
 
-Proof.
-intro E. trans (red E % #). rewrite red_mod_Frs_Decr. refl.
-rewrite rc_incl_rtc. rewrite rtc_invol. refl.
-Qed.
+  Proof.
+    intro E. trans (red E % #). rewrite red_mod_Frs_Decr. refl.
+    rewrite rc_incl_rtc. rewrite rtc_invol. refl.
+  Qed.
 
 (***********************************************************************)
 (** main theorem *)
 
-Variable Dge : relation I. Infix ">=D" := Dge (at level 50).
+  Variable Dge : relation I. Infix ">=D" := Dge (at level 50).
 
-Let Ige := IR I Dge. Infix ">=I" := Ige (at level 70).
+  Let Ige := IR I Dge. Infix ">=I" := Ige (at level 70).
 
-Variable pi_mon : forall f, Vmonotone (pi f) Dge (@Lge f).
-Variable I_mon : forall f, Vmonotone1 (fint I f) Dge.
+  Variable pi_mon : forall f, Vmonotone (pi f) Dge (@Lge f).
+  Variable I_mon : forall f, Vmonotone1 (fint I f) Dge.
 
-Section red.
+  Section red.
 
-Variable R : rules. Notation R' := (lab_rules R).
+    Variable R : rules. Notation R' := (lab_rules R).
 
-Variable ge_compat : forall l r, R (mkRule l r) -> l >=I r.
+    Variable ge_compat : forall l r, R (mkRule l r) -> l >=I r.
 
-Lemma hd_red_lab : forall v t u,
-  hd_red R t u -> hd_red_mod Decr R' (lab v t) (lab v u).
+    Lemma hd_red_lab : forall v t u,
+      hd_red R t u -> hd_red_mod Decr R' (lab v t) (lab v u).
 
-Proof.
-intros. redtac. subst. exists (lab v (sub s l)). split. apply rt_refl.
-repeat rewrite lab_sub_eq. exists (lab (beta v s) l).
-exists (lab (beta v s) r). exists (lab_sub v s). intuition.
-exists (mkRule l r). exists (beta v s). intuition.
-Qed.
+    Proof.
+      intros. redtac. subst. exists (lab v (sub s l)). split. apply rt_refl.
+      repeat rewrite lab_sub_eq. exists (lab (beta v s) l).
+      exists (lab (beta v s) r). exists (lab_sub v s). intuition.
+      exists (mkRule l r). exists (beta v s). intuition.
+    Qed.
 
-Lemma red_lab : forall v t u,
-  red R t u -> red_mod Decr R' (lab v t) (lab v u).
+    Lemma red_lab : forall v t u,
+      red R t u -> red_mod Decr R' (lab v t) (lab v u).
 
-Proof.
-intros. redtac. subst. elim c; clear c.
-(* Hole *)
-simpl. exists (lab v (sub s l)). split. apply rt_refl.
-repeat rewrite lab_sub_eq. exists (lab (beta v s) l).
-exists (lab (beta v s) r). exists Hole. exists (lab_sub v s). intuition.
-exists (mkRule l r). exists (beta v s). intuition.
-(* Cont *)
-intros. simpl. repeat rewrite Vmap_cast. repeat rewrite Vmap_app. simpl.
-set (v0' := Vmap (int v) t). set (l1 := fill c (sub s l)). fold l1 in H.
-set (v1' := Vmap (int v) t0). set (r1 := fill c (sub s r)). fold r1 in H.
-assert (int v l1 >=D int v r1). assert (IR I Dge l1 r1).
-apply IR_context_closed. hyp. apply IR_substitution_closed. apply ge_compat.
-hyp. apply H0.
-set (a := pi f (Vcast (Vapp v0' (Vcons (int v l1) v1')) e)).
-set (b := pi f (Vcast (Vapp v0' (Vcons (int v r1) v1')) e)).
-assert (a >=L b). apply pi_mon. hyp.
-set (w0 := Vmap (lab v) t). set (w1 := Vmap (lab v) t0).
-set (ts := Vcast (Vapp w0 (Vcons (lab v l1) w1)) e). ded (Lge_Decr ts H1).
-set (us := Vcast (Vapp w0 (Vcons (lab v r1) w1)) e).
-do 2 destruct H. set (vs := Vcast (Vapp w0 (Vcons x w1)) e).
-exists (Fun' (mk b) vs). split. apply rt_trans with (Fun' (mk b) ts). hyp.
-apply context_closed_fun with (R := red Decr #).
-apply context_closed_rtc. apply context_closed_red. hyp.
-apply context_closed_fun with (R := red R'). apply context_closed_red. hyp.
-Qed.
+    Proof.
+      intros. redtac. subst. elim c; clear c.
+      (* Hole *)
+      simpl. exists (lab v (sub s l)). split. apply rt_refl.
+      repeat rewrite lab_sub_eq. exists (lab (beta v s) l).
+      exists (lab (beta v s) r). exists Hole. exists (lab_sub v s). intuition.
+      exists (mkRule l r). exists (beta v s). intuition.
+      (* Cont *)
+      intros. simpl. repeat rewrite Vmap_cast. repeat rewrite Vmap_app. simpl.
+      set (v0' := Vmap (int v) t). set (l1 := fill c (sub s l)). fold l1 in H.
+      set (v1' := Vmap (int v) t0). set (r1 := fill c (sub s r)). fold r1 in H.
+      assert (int v l1 >=D int v r1). assert (IR I Dge l1 r1).
+      apply IR_context_closed. hyp. apply IR_substitution_closed.
+      apply ge_compat.
+      hyp. apply H0.
+      set (a := pi f (Vcast (Vapp v0' (Vcons (int v l1) v1')) e)).
+      set (b := pi f (Vcast (Vapp v0' (Vcons (int v r1) v1')) e)).
+      assert (a >=L b). apply pi_mon. hyp.
+      set (w0 := Vmap (lab v) t). set (w1 := Vmap (lab v) t0).
+      set (ts := Vcast (Vapp w0 (Vcons (lab v l1) w1)) e). ded (Lge_Decr ts H1).
+      set (us := Vcast (Vapp w0 (Vcons (lab v r1) w1)) e).
+      do 2 destruct H. set (vs := Vcast (Vapp w0 (Vcons x w1)) e).
+      exists (Fun' (mk b) vs). split. apply rt_trans with (Fun' (mk b) ts). hyp.
+      apply context_closed_fun with (R := red Decr #).
+      apply context_closed_rtc. apply context_closed_red. hyp.
+      apply context_closed_fun with (R := red R'). apply context_closed_red.
+      hyp.
+    Qed.
 
-Lemma rt_red_lab : forall v t u,
-  red R # t u -> red_mod Decr R' # (lab v t) (lab v u).
+    Lemma rt_red_lab : forall v t u,
+      red R # t u -> red_mod Decr R' # (lab v t) (lab v u).
 
-Proof.
-induction 1. apply rt_step. apply red_lab. hyp. apply rt_refl.
-apply rt_trans with (lab v y); hyp.
-Qed.
+    Proof.
+      induction 1. apply rt_step. apply red_lab. hyp. apply rt_refl.
+      apply rt_trans with (lab v y); hyp.
+    Qed.
 
-Lemma WF_red_lab : WF (red R) <-> WF (red_mod Decr R').
+    Lemma WF_red_lab : WF (red R) <-> WF (red_mod Decr R').
 
-Proof.
-split; intro.
-(* -> *)
-apply Fred_mod_WF with (S2:=Sig) (F:=F) (HF:=HF). apply WF_incl with (red R).
-2: hyp. intros t u h. redtac. ded (rt_red_Frs_Decr H0). subst t0. subst.
-apply red_rule. eapply Frs_iso. hyp.
-(* <- *)
-set (v := fun x : variable => some_elt I).
-apply WF_incl with (Rof (red_mod Decr R') (lab v)).
-intros t u h. unfold Rof. apply red_lab. hyp.
-apply WF_inverse. hyp.
-Qed.
+    Proof.
+      split; intro.
+      (* -> *)
+      apply Fred_mod_WF with (S2:=Sig) (F:=F) (HF:=HF).
+      apply WF_incl with (red R).
+      2: hyp. intros t u h. redtac. ded (rt_red_Frs_Decr H0). subst t0. subst.
+      apply red_rule. eapply Frs_iso. hyp.
+      (* <- *)
+      set (v := fun x : variable => some_elt I).
+      apply WF_incl with (Rof (red_mod Decr R') (lab v)).
+      intros t u h. unfold Rof. apply red_lab. hyp.
+      apply WF_inverse. hyp.
+    Qed.
 
-End red.
+  End red.
 
 (***********************************************************************)
 (** rewriting modulo *)
 
-Section red_mod.
+  Section red_mod.
 
-Variables E R : rules.
+    Variables E R : rules.
 
-Variable ge_compatE : forall l r, E (mkRule l r) -> l >=I r.
-Variable ge_compatR : forall l r, R (mkRule l r) -> l >=I r.
+    Variable ge_compatE : forall l r, E (mkRule l r) -> l >=I r.
+    Variable ge_compatR : forall l r, R (mkRule l r) -> l >=I r.
 
-Notation E' := (lab_rules E). Notation R' := (lab_rules R).
+    Notation E' := (lab_rules E). Notation R' := (lab_rules R).
 
-Lemma red_mod_lab : forall v t u,
-  red_mod E R t u -> red_mod (Decr ++ E') R' (lab v t) (lab v u).
+    Lemma red_mod_lab : forall v t u,
+      red_mod E R t u -> red_mod (Decr ++ E') R' (lab v t) (lab v u).
 
-Proof.
-intros. do 2 destruct H. ded (rt_red_lab ge_compatE v H).
-ded (red_lab ge_compatR v H0). do 2 destruct H2. exists x0. intuition.
-apply rt_trans with (lab v x).
-eapply inclusion_elim. apply rt_red_mod_union. hyp.
-eapply inclusion_elim. apply clos_refl_trans_m'. apply red_incl.
-apply incl_appl. hyp.
-Qed.
+    Proof.
+      intros. do 2 destruct H. ded (rt_red_lab ge_compatE v H).
+      ded (red_lab ge_compatR v H0). do 2 destruct H2. exists x0. intuition.
+      apply rt_trans with (lab v x).
+      eapply inclusion_elim. apply rt_red_mod_union. hyp.
+      eapply inclusion_elim. apply clos_refl_trans_m'. apply red_incl.
+      apply incl_appl. hyp.
+    Qed.
 
-Lemma hd_red_mod_lab : forall v t u,
-  hd_red_mod E R t u -> hd_red_mod (Decr ++ E') R' (lab v t) (lab v u).
+    Lemma hd_red_mod_lab : forall v t u,
+      hd_red_mod E R t u -> hd_red_mod (Decr ++ E') R' (lab v t) (lab v u).
 
-Proof.
-intros. do 2 destruct H. ded (rt_red_lab ge_compatE v H).
-ded (hd_red_lab v H0). do 2 destruct H2. exists x0. intuition.
-apply rt_trans with (lab v x).
-eapply inclusion_elim. apply rt_red_mod_union. hyp.
-eapply inclusion_elim. apply clos_refl_trans_m'. apply red_incl.
-apply incl_appl. hyp.
-Qed.
+    Proof.
+      intros. do 2 destruct H. ded (rt_red_lab ge_compatE v H).
+      ded (hd_red_lab v H0). do 2 destruct H2. exists x0. intuition.
+      apply rt_trans with (lab v x).
+      eapply inclusion_elim. apply rt_red_mod_union. hyp.
+      eapply inclusion_elim. apply clos_refl_trans_m'. apply red_incl.
+      apply incl_appl. hyp.
+    Qed.
 
-Lemma WF_red_mod_lab : WF (red_mod E R) <-> WF (red_mod (Decr ++ E') R').
+    Lemma WF_red_mod_lab : WF (red_mod E R) <-> WF (red_mod (Decr ++ E') R').
 
-Proof.
-split; intro.
-(* -> *)
-apply Fred_mod_WF with (S2:=Sig) (F:=F) (HF:=HF).
-apply WF_incl with (red_mod E R). 2: hyp. intros t u h. destruct h.
-destruct H0. apply rt_red_mod_Frs_Decr in H0. rewrite Frs_iso in H1.
-exists x. auto.
-(* <- *)
-set (v := fun x : variable => some_elt I).
-apply WF_incl with (Rof (red_mod (Decr ++ E') R') (lab v)).
-intros t u h. unfold Rof. apply red_mod_lab. hyp.
-apply WF_inverse. hyp.
-Qed.
+    Proof.
+      split; intro.
+      (* -> *)
+      apply Fred_mod_WF with (S2:=Sig) (F:=F) (HF:=HF).
+      apply WF_incl with (red_mod E R). 2: hyp. intros t u h. destruct h.
+      destruct H0. apply rt_red_mod_Frs_Decr in H0. rewrite Frs_iso in H1.
+      exists x. auto.
+      (* <- *)
+      set (v := fun x : variable => some_elt I).
+      apply WF_incl with (Rof (red_mod (Decr ++ E') R') (lab v)).
+      intros t u h. unfold Rof. apply red_mod_lab. hyp.
+      apply WF_inverse. hyp.
+    Qed.
 
-Lemma WF_hd_red_mod_lab :
-  WF (hd_red_mod E R) <-> WF (hd_red_mod (Decr ++ E') R').
+    Lemma WF_hd_red_mod_lab :
+      WF (hd_red_mod E R) <-> WF (hd_red_mod (Decr ++ E') R').
 
-Proof.
-split; intro.
-(* -> *)
-apply Fhd_red_mod_WF with (S2:=Sig) (F:=F) (HF:=HF).
-apply WF_incl with (hd_red_mod E R). 2: hyp. intros t u h. destruct h.
-destruct H0. apply rt_red_mod_Frs_Decr in H0. rewrite Frs_iso in H1.
-exists x. auto.
-(* <- *)
-set (v := fun x : variable => some_elt I).
-apply WF_incl with (Rof (hd_red_mod (Decr ++ E') R') (lab v)).
-intros t u h. unfold Rof. apply hd_red_mod_lab. hyp.
-apply WF_inverse. hyp.
-Qed.
+    Proof.
+      split; intro.
+      (* -> *)
+      apply Fhd_red_mod_WF with (S2:=Sig) (F:=F) (HF:=HF).
+      apply WF_incl with (hd_red_mod E R). 2: hyp. intros t u h. destruct h.
+      destruct H0. apply rt_red_mod_Frs_Decr in H0. rewrite Frs_iso in H1.
+      exists x. auto.
+      (* <- *)
+      set (v := fun x : variable => some_elt I).
+      apply WF_incl with (Rof (hd_red_mod (Decr ++ E') R') (lab v)).
+      intros t u h. unfold Rof. apply hd_red_mod_lab. hyp.
+      apply WF_inverse. hyp.
+    Qed.
 
-End red_mod.
+  End red_mod.
 
 (***********************************************************************)
 (** enumeration of labelled rules for a finite domain *)
 
-Section enum.
+  Section enum.
 
-Variable Is : list I.
-Variable Is_ok : forall x : I, In x Is.
+    Variable Is : list I.
+    Variable Is_ok : forall x : I, In x Is.
 
-Fixpoint enum_tuple n : list (vector I n) :=
-  match n with
-    | 0 => cons Vnil nil
-    | S p => flat_map (fun ds => map (fun d => Vcons d ds) Is) (enum_tuple p)
-  end.
+    Fixpoint enum_tuple n : list (vector I n) :=
+      match n with
+        | 0 => cons Vnil nil
+        | S p =>
+          flat_map (fun ds => map (fun d => Vcons d ds) Is) (enum_tuple p)
+      end.
 
-Lemma enum_tuple_complete : forall n (ds : vector I n), In ds (enum_tuple n).
+    Lemma enum_tuple_complete : forall n (ds : vector I n),
+      In ds (enum_tuple n).
 
-Proof.
-induction n; simpl; intros. VOtac. auto. rewrite in_flat_map.
-exists (Vtail ds). split. apply IHn.
-set (f := fun d : I => Vcons d (Vtail ds)).
-VSntac ds. change (In (f (Vhead ds)) (map f Is)). apply in_map. apply Is_ok.
-Qed.
+    Proof.
+      induction n; simpl; intros. VOtac. auto. rewrite in_flat_map.
+      exists (Vtail ds). split. apply IHn.
+      set (f := fun d : I => Vcons d (Vtail ds)).
+      VSntac ds. change (In (f (Vhead ds)) (map f Is)). apply in_map.
+      apply Is_ok.
+    Qed.
 
 (*REMARK: define a more efficient function?
 Fixpoint enum_tuple2 n : list (vector I n) :=
@@ -440,35 +447,33 @@ Fixpoint enum_tuple2 n : list (vector I n) :=
       (enum_tuple2 p) nil
   end.*)
 
-Definition enum R :=
-  flat_map (fun ds => map (lab_rule (val_of_vec I ds)) R)
-  (enum_tuple (S (maxvar_rules R))).
+    Definition enum R :=
+      flat_map (fun ds => map (lab_rule (val_of_vec I ds)) R)
+      (enum_tuple (S (maxvar_rules R))).
 
-Lemma enum_correct : forall R a, In a (enum R) -> lab_rules (Rules R) a.
+    Lemma enum_correct : forall R a, In a (enum R) -> lab_rules (Rules R) a.
 
-Proof.
-intros. unfold enum in H. rewrite in_flat_map in H. do 2 destruct H.
-rewrite in_map_iff in H0. do 2 destruct H0. exists x0. exists (val_of_vec I x).
-intuition.
-Qed.
+    Proof.
+      intros. unfold enum in H. rewrite in_flat_map in H. do 2 destruct H.
+      rewrite in_map_iff in H0. do 2 destruct H0. exists x0.
+      exists (val_of_vec I x). intuition.
+    Qed.
 
-Lemma enum_complete : forall R a, lab_rules (Rules R) a -> In a (enum R).
+    Lemma enum_complete : forall R a, lab_rules (Rules R) a -> In a (enum R).
 
-Proof.
-intros. do 3 destruct H. set (n := maxvar_rules R).
-unfold enum. rewrite in_flat_map. exists (vec_of_val x0 (S n)). split.
-apply enum_tuple_complete. subst.
-change (In (lab_rule x0 x) (map (lab_rule (fval x0 (S n))) R)).
-rewrite map_lab_rule_fval. apply in_map. hyp. unfold n. omega.
-Qed.
+    Proof.
+      intros. do 3 destruct H. set (n := maxvar_rules R).
+      unfold enum. rewrite in_flat_map. exists (vec_of_val x0 (S n)). split.
+      apply enum_tuple_complete. subst.
+      change (In (lab_rule x0 x) (map (lab_rule (fval x0 (S n))) R)).
+      rewrite map_lab_rule_fval. apply in_map. hyp. unfold n. omega.
+    Qed.
 
-Infix "[=]" := equiv.
+    Infix "[=]" := equiv.
 
-Lemma lab_rules_enum : forall R, lab_rules (Rules R) [=] Rules (enum R).
+    Lemma lab_rules_enum : forall R, lab_rules (Rules R) [=] Rules (enum R).
 
-Proof.
-split. apply enum_complete. apply enum_correct.
-Qed.
+    Proof. split. apply enum_complete. apply enum_correct. Qed.
 
 (*REMARK: define a more efficient function?
 Definition enum2 R :=
@@ -483,144 +488,146 @@ Definition enum2 R :=
 (***********************************************************************)
 (** enumeration of labelled symbols *)
 
-Variable Fs : list Sig.
-Variable Fs_ok : forall x, In x Fs.
+    Variable Fs : list Sig.
+    Variable Fs_ok : forall x, In x Fs.
 
-Variable Ls : forall f, list (L f).
-Variable Ls_ok : forall f (x : L f), In x (Ls f).
+    Variable Ls : forall f, list (L f).
+    Variable Ls_ok : forall f (x : L f), In x (Ls f).
 
-Definition Fs_lab := flat_map (fun f => map (@mk f) (Ls f)) Fs.
+    Definition Fs_lab := flat_map (fun f => map (@mk f) (Ls f)) Fs.
 
-Lemma Fs_lab_ok : forall f : Sig', In f Fs_lab.
+    Lemma Fs_lab_ok : forall f : Sig', In f Fs_lab.
 
-Proof.
-intros [f l]. unfold Fs_lab. rewrite in_flat_map. exists f. split.
-apply Fs_ok. rewrite in_map_iff. exists l. intuition.
-Qed.
+    Proof.
+      intros [f l]. unfold Fs_lab. rewrite in_flat_map. exists f. split.
+      apply Fs_ok. rewrite in_map_iff. exists l. intuition.
+    Qed.
 
 (***********************************************************************)
 (** enumeration of Decr rules *)
 
-Variable L2s : forall f, list (L f * L f).
-Variable L2s_ok : forall f (x y : L f), x >L y <-> In (x,y) (L2s f).
+    Variable L2s : forall f, list (L f * L f).
+    Variable L2s_ok : forall f (x y : L f), x >L y <-> In (x,y) (L2s f).
 
-Definition enum_Decr := flat_map (fun f =>
-  map (fun x : L f * L f => let (a,b) := x in decr a b) (L2s f)) Fs.
+    Definition enum_Decr := flat_map (fun f =>
+      map (fun x : L f * L f => let (a,b) := x in decr a b) (L2s f)) Fs.
 
-Notation D' := enum_Decr.
+    Notation D' := enum_Decr.
 
-Lemma enum_Decr_correct : forall x, In x D' -> Decr x.
+    Lemma enum_Decr_correct : forall x, In x D' -> Decr x.
 
-Proof.
-intros. unfold enum_Decr in H. rewrite in_flat_map in H.
-destruct H as [f]. destruct H. rewrite in_map_iff in H0.
-destruct H0 as [[a b]]. destruct H0. exists f. exists a. exists b.
-rewrite L2s_ok. auto.
-Qed.
+    Proof.
+      intros. unfold enum_Decr in H. rewrite in_flat_map in H.
+      destruct H as [f]. destruct H. rewrite in_map_iff in H0.
+      destruct H0 as [[a b]]. destruct H0. exists f. exists a. exists b.
+      rewrite L2s_ok. auto.
+    Qed.
 
-Lemma enum_Decr_complete : forall x, Decr x -> In x D'.
+    Lemma enum_Decr_complete : forall x, Decr x -> In x D'.
 
-Proof.
-intros. destruct H as [f [a [b [h]]]]. unfold enum_Decr. rewrite in_flat_map.
-exists f. split. apply Fs_ok. rewrite in_map_iff. exists (a,b).
-rewrite <- L2s_ok. auto.
-Qed.
+    Proof.
+      intros. destruct H as [f [a [b [h]]]]. unfold enum_Decr.
+      rewrite in_flat_map.
+      exists f. split. apply Fs_ok. rewrite in_map_iff. exists (a,b).
+      rewrite <- L2s_ok. auto.
+    Qed.
 
-Lemma Rules_enum_Decr : Rules D' [=] Decr.
+    Lemma Rules_enum_Decr : Rules D' [=] Decr.
 
-Proof.
-unfold equiv. split; intro. apply enum_Decr_correct. hyp.
-apply enum_Decr_complete. hyp.
-Qed.
+    Proof.
+      unfold equiv. split; intro. apply enum_Decr_correct. hyp.
+      apply enum_Decr_complete. hyp.
+    Qed.
 
 (***********************************************************************)
 (** main theorems (finite versions) *)
 
-Import ATrs. Notation rules := (rules Sig).
+    Import ATrs. Notation rules := (rules Sig).
 
-Variable bge : term -> term -> bool.
-Variable bge_ok : rel bge << Ige.
+    Variable bge : term -> term -> bool.
+    Variable bge_ok : rel bge << Ige.
 
-Section bge.
+    Section bge.
 
-Variable R : rules.
-Variable bge_compat : forallb (brule bge) R = true.
+      Variable R : rules.
+      Variable bge_compat : forallb (brule bge) R = true.
 
-Lemma ge_compat : forall l r, In (mkRule l r) R -> l >=I r.
+      Lemma ge_compat : forall l r, In (mkRule l r) R -> l >=I r.
 
-Proof.
-intros. apply bge_ok. unfold rel. change (brule bge (mkRule l r) = true).
-rewrite forallb_forall in bge_compat. apply bge_compat. hyp.
-Qed.
+      Proof.
+        intros. apply bge_ok. unfold rel.
+        change (brule bge (mkRule l r) = true).
+        rewrite forallb_forall in bge_compat. apply bge_compat. hyp.
+      Qed.
 
-End bge.
+    End bge.
 
-Implicit Arguments ge_compat [R].
+    Implicit Arguments ge_compat [R].
 
-Section red_mod.
+    Section red_mod.
 
-Variables E R : rules.
+      Variables E R : rules.
 
-Notation E' := (enum E). Notation R' := (enum R).
+      Notation E' := (enum E). Notation R' := (enum R).
 
-Variable bge_compatE : forallb (brule bge) E = true.
-Variable bge_compatR : forallb (brule bge) R = true.
+      Variable bge_compatE : forallb (brule bge) E = true.
+      Variable bge_compatR : forallb (brule bge) R = true.
 
-Notation ge_compatE := (ge_compat bge_compatE).
-Notation ge_compatR := (ge_compat bge_compatR).
+      Notation ge_compatE := (ge_compat bge_compatE).
+      Notation ge_compatR := (ge_compat bge_compatR).
 
-Lemma WF_red_lab_fin : WF (red R) <-> WF (red_mod D' R').
+      Lemma WF_red_lab_fin : WF (red R) <-> WF (red_mod D' R').
 
-Proof.
-rewrite <- red_Rules. rewrite <- red_mod_Rules. rewrite WF_red_lab.
-2: apply ge_compatR. apply WF_m. rewrite Rules_enum_Decr.
-rewrite lab_rules_enum. refl.
-Qed.
+      Proof.
+        rewrite <- red_Rules. rewrite <- red_mod_Rules. rewrite WF_red_lab.
+        2: apply ge_compatR. apply WF_m. rewrite Rules_enum_Decr.
+        rewrite lab_rules_enum. refl.
+      Qed.
 
-Import List.
+      Import List.
 
-Lemma WF_red_mod_lab_fin : WF (red_mod E R) <-> WF (red_mod (D' ++ E') R').
+      Lemma WF_red_mod_lab_fin :
+        WF (red_mod E R) <-> WF (red_mod (D' ++ E') R').
 
-Proof.
-repeat rewrite <- red_mod_Rules. rewrite WF_red_mod_lab.
-2: apply ge_compatE. 2: apply ge_compatR.
-apply WF_m. rewrite Rules_app. rewrite Rules_enum_Decr.
-repeat rewrite lab_rules_enum. refl.
-Qed.
+      Proof.
+        repeat rewrite <- red_mod_Rules. rewrite WF_red_mod_lab.
+        2: apply ge_compatE. 2: apply ge_compatR.
+        apply WF_m. rewrite Rules_app. rewrite Rules_enum_Decr.
+        repeat rewrite lab_rules_enum. refl.
+      Qed.
 
-Lemma WF_hd_red_mod_lab_fin :
-  WF (hd_red_mod E R) <-> WF (hd_red_mod (D' ++ E') R').
+      Lemma WF_hd_red_mod_lab_fin :
+        WF (hd_red_mod E R) <-> WF (hd_red_mod (D' ++ E') R').
 
-Proof.
-repeat rewrite <- hd_red_mod_Rules. rewrite WF_hd_red_mod_lab.
-2: apply ge_compatE. apply WF_m. rewrite Rules_app. rewrite Rules_enum_Decr.
-repeat rewrite lab_rules_enum. refl.
-Qed.
+      Proof.
+        repeat rewrite <- hd_red_mod_Rules. rewrite WF_hd_red_mod_lab.
+        2: apply ge_compatE. apply WF_m. rewrite Rules_app, Rules_enum_Decr.
+        repeat rewrite lab_rules_enum. refl.
+      Qed.
 
-End red_mod.
+    End red_mod.
 
-Lemma WF_red_unlab_fin : forall R, WF (red (unlab_rules_fin R)) -> WF (red R).
+    Lemma WF_red_unlab_fin : forall R,
+      WF (red (unlab_rules_fin R)) -> WF (red R).
 
-Proof.
-intros. apply Fred_WF_fin with (S2:=Sig) (F:=F) (HF:=HF). hyp.
-Qed.
+    Proof. intros. apply Fred_WF_fin with (S2:=Sig) (F:=F) (HF:=HF). hyp. Qed.
 
-Lemma WF_red_mod_unlab_fin : forall E R,
-  WF (red_mod (unlab_rules_fin E) (unlab_rules_fin R)) -> WF (red_mod E R).
+    Lemma WF_red_mod_unlab_fin : forall E R,
+      WF (red_mod (unlab_rules_fin E) (unlab_rules_fin R)) -> WF (red_mod E R).
 
-Proof.
-intros. apply Fred_mod_WF_fin with (S2:=Sig) (F:=F) (HF:=HF). hyp.
-Qed.
+    Proof.
+      intros. apply Fred_mod_WF_fin with (S2:=Sig) (F:=F) (HF:=HF). hyp.
+    Qed.
 
-Lemma WF_hd_red_mod_unlab_fin : forall E R,
-  WF (hd_red_mod (unlab_rules_fin E) (unlab_rules_fin R))
-  -> WF (hd_red_mod E R).
+    Lemma WF_hd_red_mod_unlab_fin : forall E R,
+      WF (hd_red_mod (unlab_rules_fin E) (unlab_rules_fin R))
+      -> WF (hd_red_mod E R).
 
-Proof.
-intros. apply Fhd_red_mod_WF_fin with (S2:=Sig) (F:=F) (HF:=HF). hyp.
-Qed.
+    Proof.
+      intros. apply Fhd_red_mod_WF_fin with (S2:=Sig) (F:=F) (HF:=HF). hyp.
+    Qed.
 
-End enum.
+  End enum.
 
 End S.
 
@@ -710,9 +717,7 @@ Module Ord (SL : SemLab) <: OrdSemLab.
 
   Lemma Lge_is_eq : forall f a b, (@Lgt f%) a b <-> a = b.
 
-  Proof.
-    fo.
-  Qed.
+  Proof. fo. Qed.
 
   Lemma pi_mon : forall f, Vmonotone (pi f) Dge (@Lgt f%).
 
@@ -727,9 +732,7 @@ Module Ord (SL : SemLab) <: OrdSemLab.
 
   Lemma Decr_empty : Decr beq_ok Lgt [=] @empty (@ATrs.rule Sig').
 
-  Proof.
-    fo.
-  Qed.
+  Proof. fo. Qed.
 
 End Ord.
 
@@ -792,9 +795,7 @@ Module FinOrd (Import FSL : FinSemLab) <: FinOrdSemLab.
 
   Lemma L2s_ok : forall f (x y : L f), Lgt x y <-> In (x,y) (L2s f).
 
-  Proof.
-    fo.
-  Qed.
+  Proof. fo. Qed.
 
   Lemma enum_Decr_empty : enum_Decr beq_ok Fs L2s = nil.
 
